extraction/theories/OptimizePropDiscr.v
@@ -1,0 +1,51 @@
+(* Pass that removes discrimination (matches and projections) on things in Prop.
+   This uses MetaCoq's optimization but adapted to run on our environments. *)
+
+From ConCert.Extraction Require Import ExAst.
+From MetaCoq.Erasure Require Import EOptimizePropDiscr.
+From MetaCoq.Erasure Require Import EWcbvEval.
+
+Definition optimize_constant_body Σ cst :=
+  {| cst_type := cst_type cst;
+     cst_body := option_map (optimize Σ) (cst_body cst) |}.
+
+Definition optimize_decl Σ d :=
+  match d with
+  | ConstantDecl cst => ConstantDecl (optimize_constant_body Σ cst)
+  | _ => d
+  end.
+
+Definition optimize_env (Σ : global_env) : global_env :=
+  map (on_snd (optimize_decl (trans_env Σ))) Σ.
+
+Module Ee := EWcbvEval.
+
+Lemma trans_env_optimize_env Σ :
+  trans_env (optimize_env Σ) =
+  EOptimizePropDiscr.optimize_env (trans_env Σ).
+Proof.
+  unfold trans_env.
+  unfold EOptimizePropDiscr.optimize_env.
+  unfold optimize_env.
+  rewrite !map_map.
+  apply map_ext.
+  intros ((kn&has_deps)&decl).
+  cbn.
+  f_equal.
+  destruct decl; auto.
+  cbn.
+  now destruct o.
+Qed.
+
+Lemma optimize_correct Σ t v :
+  @Ee.eval Ee.default_wcbv_flags (trans_env Σ) t v ->
+  @Ee.eval
+      Ee.opt_wcbv_flags
+      (trans_env (optimize_env Σ))
+      (optimize (trans_env Σ) t)
+      (optimize (trans_env Σ) v).
+Proof.
+  intros ev.
+  rewrite trans_env_optimize_env.
+  now apply EOptimizePropDiscr.optimize_correct.
+Qed.
