extraction/theories/Transform.v
@@ -1,0 +1,35 @@
+From ConCert.Extraction Require Import ExAst.
+From ConCert.Extraction Require Import ResultMonad.
+From ConCert.Extraction Require Import WcbvEvalAux.
+From Equations Require Import Equations.
+From MetaCoq.Template Require Import utils.
+
+Definition Transform := global_env -> result global_env string.
+Definition TransformCorrect (transform : Transform) : Type :=
+  forall Σ Σopt kn ind c (wf := EWcbvEval.opt_wcbv_flags),
+    transform Σ = Ok Σopt ->
+    trans_env Σ e⊢ tConst kn ▷ tConstruct ind c ->
+    trans_env Σopt e⊢ tConst kn ▷ tConstruct ind c.
+
+Definition CorrectTransform := ∑ t, TransformCorrect t.
+
+Fixpoint compose_transforms (transforms : list Transform) : Transform :=
+  match transforms with
+  | [] => Ok
+  | t :: transforms =>
+    fun Σ =>
+      Σopt <- t Σ;;
+      compose_transforms transforms Σopt
+  end.
+
+Lemma compose_transforms_correct transforms :
+  All TransformCorrect transforms ->
+  TransformCorrect (compose_transforms transforms).
+Proof.
+  intros all Σ Σopt kn ind c wf success ev.
+  subst wf.
+  induction all in Σ, success, ev |- *; cbn in *.
+  - now injection success as ->.
+  - destruct x eqn:teq; [|congruence].
+    eapply (p _ _ kn ind c) in teq; eauto.
+Qed.
